Add demand specification

src/BankersQueue.v
@@ -19,9 +19,10 @@ From Equations Require Import Equations.
 
 From Coq Require Import Arith List Lia Setoid Morphisms.
 Import ListNotations.
-From Clairvoyance Require Import Core Approx ApproxM List Misc.
+From Clairvoyance Require Import Core Approx ApproxM List Misc Tick.
 
 Import RevCompare.
+Import Tick.Notations.
 
 Set Primitive Projections.
 Set Implicit Arguments.
@@ -324,54 +325,6 @@ Proof.
   - rewrite (frontn wf_q), Ef. reflexivity.
   - apply (backn wf_q).
 Qed.
-
-(** * The tick monad *)
-
-Module Tick.
-
-Record Tick (a : Type) : Type := MkTick
-  { cost : nat
-  ; val : a
-  }.
-
-Arguments MkTick {a}.
-Arguments cost {a}.
-Arguments val {a}.
-
-Definition ret {a} : a -> Tick a := MkTick 0.
-Definition bind {a b} (u : Tick a) (k : a -> Tick b) : Tick b :=
-  {| cost := cost u + cost (k (val u))
-  ;  val := val (k (val u))
-  |}.
-
-Definition tick : Tick unit := MkTick 1 tt.
-
-Module Notations.
-Declare Scope tick_scope.
-Delimit Scope tick_scope with tick.
-Bind Scope tick_scope with Tick.
-
-Notation "'let+' x := u 'in' k" := (bind u (fun x => k%tick))
-  (at level 200, x as pattern) : tick_scope.
-Notation "u >> v" := (bind u (fun _ => v%tick)) : tick_scope.
-
-End Notations.
-
-#[global] Instance LessDefined_Tick {a} `{LessDefined a} : LessDefined (Tick a) :=
-  fun x y => cost x <= cost y /\ val x `less_defined` val y.
-
-#[global] Instance Transitive_LessDefined_Tick {a} `{LessDefined a}
-  `{!Transitive (less_defined (a := a))} : Transitive (less_defined (a := Tick a)).
-Proof.
-  unfold Transitive, less_defined, LessDefined_Tick; intros * [] []; split; etransitivity; eauto.
-Qed.
-
-#[global] Instance Bottom_Tick {a} `{Bottom a} : Bottom (Tick a) := MkTick 0 bottom.
-
-End Tick.
-Notation Tick := Tick.Tick.
-
-Import Tick.Notations.
 
 (** * Demand *)
 
