src/Tick.v
@@ -1,0 +1,50 @@
+(** * The tick monad *)
+
+From Clairvoyance Require Import Approx.
+From Coq Require Import Morphisms.
+
+Set Primitive Projections.
+
+Module Tick.
+
+Record Tick (a : Type) : Type := MkTick
+  { cost : nat
+  ; val : a
+  }.
+
+Arguments MkTick {a}.
+Arguments cost {a}.
+Arguments val {a}.
+
+Definition ret {a} : a -> Tick a := MkTick 0.
+Definition bind {a b} (u : Tick a) (k : a -> Tick b) : Tick b :=
+  {| cost := cost u + cost (k (val u))
+  ;  val := val (k (val u))
+  |}.
+
+Definition tick : Tick unit := MkTick 1 tt.
+
+Module Notations.
+Declare Scope tick_scope.
+Delimit Scope tick_scope with tick.
+Bind Scope tick_scope with Tick.
+
+Notation "'let+' x := u 'in' k" := (bind u (fun x => k%tick))
+  (at level 200, x as pattern) : tick_scope.
+Notation "u >> v" := (bind u (fun _ => v%tick)) (at level 61, left associativity) : tick_scope.
+
+End Notations.
+
+#[global] Instance LessDefined_Tick {a} `{LessDefined a} : LessDefined (Tick a) :=
+  fun x y => cost x <= cost y /\ val x `less_defined` val y.
+
+#[global] Instance Transitive_LessDefined_Tick {a} `{LessDefined a}
+  `{!Transitive (less_defined (a := a))} : Transitive (less_defined (a := Tick a)).
+Proof.
+  unfold Transitive, less_defined, LessDefined_Tick; intros * [] []; split; etransitivity; eauto.
+Qed.
+
+#[global] Instance Bottom_Tick {a} `{Bottom a} : Bottom (Tick a) := MkTick 0 bottom.
+
+End Tick.
+Notation Tick := Tick.Tick.
